\def\module{M3P11 Galois Theory}
\def\lecturer{Prof Alessio Corti}
\def\term{Spring 2019}

\def\thm{section}

\input{../style/header}

\begin{document}

\input{../style/main}

\section{What is Galois theory?}

\lecture{1}{Thursday}{10/01/19}

The following are references.
\begin{itemize}
\item E Artin, Galois theory, 1994
\item A Grothendieck and M Raynaud, Rev\^etements \'etales et groupe fondamental, 2002
\item I N Herstein, Topics in algebra, 1975
\item M Reid, Galois theory, 2014
\end{itemize}

\begin{notation*}
If $ K $ is a field, or a ring, I denote
$$ K\sb{x} = \cb{a_0 + \dots + a_nx^n \mid a_i \in K}, $$
the ring of polynomials with coefficients in $ K $.
\end{notation*}

\begin{example*}
\hfill
\begin{itemize}
\item $ \Q, \R, \C $.
\item Quadratic fields
$$ \Q\rb{\sqrt{2}} = \cb{a + b\sqrt{2} \mid a, b \in \Q} = \dfrac{\Q\sb{x}}{\ab{x^2 - 2}}. $$
It is also a field, since
$$ \dfrac{1}{\rb{a + b\sqrt{2}}} = \dfrac{a - b\sqrt{2}}{a^2 - 2b^2}. $$
\item If $ p $ is prime, $ \Z / p\Z = \F_p $ is a finite field. If $ f\rb{x} \in K\sb{x} $ is irreducible, $ K\sb{x} / \ab{f\rb{x}} $ is a field. For example, $ x^2 - 2 $. Both $ \Z $ and $ K\sb{x} $ have a division algorithm. For example, let $ \sb{a} \in \Z / p\Z $ and $ \sb{a} \ne 0 $, that is $ p \mid a $. Since $ p $ is prime, $ \gcd\rb{p, a} = 1 $, so there exist $ x, y \in \Z $ such that $ ax + py = 1 $. Thus $ \sb{a} \cdot \sb{x} = 1 $ in $ \Z / p\Z $.
\item For $ K $ a field, either for all $ m \in \Z $, $ m \ne 0 $ in $ K $, so $ K $ has characteristic $ ch\rb{K} = 0 $, or there exists $ p $ prime such that $ m = 0 $ if and only if $ p \mid m $, so $ K $ has characteristic $ ch\rb{K} = p $.
\item For $ K $ a field,
$$ K\rb{x} = Frac\rb{K\sb{x}} = \cb{\phi\rb{x} = \dfrac{f\rb{x}}{g\rb{x}} \ \Bigg| \ f, g \in K\sb{x}, \ g \ne 0}. $$
is also a field, the field of rational functions with coefficients in $ K $. For example, $ \F_p\rb{x, Y} = \F_p\rb{x}\rb{Y} $.
\end{itemize}
\end{example*}

\begin{example*}
Consider algebraic equations in a field $ K $.
\begin{itemize}
\item Let $ ax^2 + bx^2 + c = 0 $ for $ a, b, c \in K $ be a quadratic. There is a formula
$$ x = \dfrac{-b + \sqrt{b^2 - 4ac}}{2a}. $$
\item For a cubic $ y^3 + 3py + 2q = 0 $,
$$ y = \sqrt[3]{-q + \sqrt{q^2 + p^3}} + \sqrt[3]{-q - \sqrt{q^2 + p^3}}. $$
\item There is a formula for quartic equations.
\item It is a theorem that there can be no such formula for equations of degree at least five.
\end{itemize}
Galois theory deals with these easily.
\end{example*}

\lecture{2}{Friday}{11/01/19}

\begin{definition}
A \textbf{field homomorphism} is a function $ \phi : K_1 \to K_2 $ that preserves the field operations, for all $ a, b \in K_1 $,
\begin{align*}
\phi\rb{a + b} & = \phi\rb{a} + \phi\rb{b}, \\
\phi\rb{ab} & = \phi\rb{a}\phi\rb{b},
\end{align*}
and $ \phi\rb{0_{K_1}} = 0_{K_2} $ and $ \phi\rb{1_{K_1}} = 1_{K_2} $.
\end{definition}

\begin{remark*}
All field homomorphisms are injective. If $ a \in K_1 \setminus \cb{0} $, then there exists $ b \in K_1 $ such that $ ab = 1 $, then $ \phi\rb{a}\phi\rb{b} = 1 $, so $ \phi\rb{a} \ne 0 $. This easily implies $ \phi $ is injective. If $ a_1 \ne a_2 $, then $ a_1 - a_n \ne 0 $, so $ 0 \ne \phi\rb{a_1 - a_2} = \phi\rb{a_1} - \phi\rb{a_2} $. Then $ \phi\rb{a_1} \ne \phi\rb{a_2} $.
\end{remark*}

We concern ourselves with field extensions $ k \subset K $, and every homomorphism is an extension. Consider a field extension $ k \subset K $ and $ \alpha \in K $. Then $ k\rb{\alpha} \subset K $ denotes the smallest subfield of $ K $ that contains $ k, \alpha $. Not to be confused with $ k\rb{x} $.

\begin{example*}
There are two very different cases exemplified in $ \Q \subset \C $.
\begin{itemize}
\item $ \alpha = \sqrt{2} $, $ \Q\rb{\sqrt{2}} $.
\item $ \alpha = \pi $, $ \Q\rb{\pi} $.
\end{itemize}
\end{example*}

\begin{definition}
\hfill
\begin{itemize}
\item $ \alpha $ is \textbf{algebraic} over $ k $ if $ f\rb{\alpha} = 0 $ for some $ 0 \ne f \in k\sb{x} $. Otherwise we say that $ \alpha $ is \textbf{transcendental} over $ k $.
\item The extension $ k \subset K $ is \textbf{algebraic} if for all $ \alpha \in K $, $ \alpha $ is algebraic over $ k $.
\end{itemize}
\end{definition}

\begin{definition}
Consider a field $ k $ and $ f \in k\sb{x} $. We say that $ k \subset K $ is a \textbf{splitting field} for $ f $ if
\begin{itemize}
\item $ f\rb{x} = a\prod_{i = 1}^n \rb{x - \lambda_i} \in K\sb{x} $ for $ a \in k \setminus \cb{0} $, and
\item $ K = k\rb{\lambda_1, \dots, \lambda_n} $.
\end{itemize}

\end{definition}

\begin{example*}
\hfill
\begin{itemize}
\item If $ f\rb{x} = x^2 - 2 \in \Q\sb{x} $, then $ K = \Q\rb{\sqrt{2}} $ is a splitting field for $ f $. Indeed
$$ x^2 - 2 =\rb{x + \sqrt{2}}\rb{x - \sqrt{2}} \in \Q\rb{\sqrt{2}}\sb{x}. $$
\item If $ f\rb{x} = x^2 + 2 $, then $ K = \Q\rb{\sqrt{-2}} $.
\item If $ f\rb{x} = x^3 - 2 $, then
$$ \Q\rb{\sqrt[3]{2}} = \cb{a + b\sqrt[3]{2} + c\sqrt[3]{4} \mid a, b, c \in \Q} $$
is not a splitting field. $ K = \Q\rb{\sqrt[3]{2}, \omega} $, where $ \omega = \tfrac{-1 + \sqrt{3}}{2} $, is a splitting field.
$$ x^3 - 2 = \rb{x - \sqrt[3]{2}}\rb{x - \omega\sqrt[3]{2}}\rb{x - \omega^2\sqrt[3]{2}}. $$
\end{itemize}
\end{example*}

\pagebreak

\begin{theorem}[Fundamental theorem of Galois theory]
\label{thm:galoiscorrespondence}
Assume characteristic zero. Let $ k \subset K $ be the splitting field of $ f\rb{x} \in k\sb{x} $. Let
$$ G = \cb{\sigma : K \to K \mid \sigma \ \text{field automorphism}, \ \sigma\mid_{k} = id_k}. $$
We call this group the \textbf{Galois group}. There is a one-to-one correspondence
$$
\begin{array}{rcl}
\cb{k \subset K_1 \subset K \mid K_1 \ \text{subfield}} & \leftrightarrow & \cb{H \le G \mid H \ \text{subgroup}} \\
K_1 & \mapsto & \cb{\sigma \in G \mid \forall \lambda \in K_1, \ \sigma\rb{\lambda} = \lambda} \\
\cb{\lambda \in K \mid \forall \sigma \in H, \ \sigma\rb{\lambda} = \lambda} & \mapsfrom & H \le G.
\end{array}.
$$
\end{theorem}

Why is this cool? Fields are hard, groups are easy. We will see that there is a good formula for the roots of $ f\rb{x} $ if and only if $ G $ is a soluble group.

\lecture{3}{Tuesday}{15/01/19}

\begin{example*}
Let $ \deg\rb{f} = 2 $ and $ f\rb{x} = x^2 + 2Ax + B \in K\sb{x} $. If $ K $ already contains the roots then $ L = K $ and $ G = \cb{id} $. Suppose $ K $ does not contain the roots. We still have quadratic formula
$$ \lambda_{1, 2} = -A \pm \sqrt{A^2 - B}. $$
If $ \Delta = A^2 - B $ then $ \sqrt{\Delta} $ does not exist in $ K $. We must have
$$ L = K\rb{\sqrt{\Delta}} = \cb{a + b\sqrt{\Delta} \mid a, b \in K}. $$
Then $ K \subset L $ and
$$ G = \cb{\sigma : L \to L \mid \sigma \mid_K = id_K} = C_2 $$
is generated by
$$ \sigma : a + b\sqrt{\Delta} \mapsto a - b\sqrt{\Delta}. $$
Further specialisation is the following.
\begin{itemize}
\item Let $ K = \R $ and $ \Delta = -1 $. Then
$$ L = \C = \cb{a + b\sqrt{-1} \mid a, b \in \R}, $$
and $ G = C_2 $ is generated by
$$ \sigma : a + b\sqrt{-1} \mapsto a - b\sqrt{-1}, $$
complex conjugation.
\item Let $ K = \Q $ and $ \Delta = 2 $. Then
$$ L = \cb{a + b\sqrt{2} \mid a, b \in \Q}, $$
and $ G = C_2 $ is generated by
$$ \sigma : a + b\sqrt{2} \mapsto a - b\sqrt{2}. $$
\end{itemize}
The fundamental theorem implies there does not exist
$$ K \subsetneq K_1 \subsetneq K\rb{\sqrt{\Delta}} = L. $$
Is this obvious? Consider $ x \in L \setminus K $, so $ x = a + b\sqrt{\Delta} $, and $ b \ne 0 $, and then
$$ \sqrt{\Delta} = \dfrac{x - a}{b}, $$
so $ K\rb{x} = L $.
\end{example*}

\begin{example*}
Let $ f\rb{x} = x^3 - 2 \in \Q\sb{x} $ and $ L = \Q\rb{\sqrt[3]{2}, \omega} $, where $ \omega = \tfrac{-1 + i\sqrt{3}}{2} $ is a solution of $ x^2 + x + 1 = 0 $. Then
$$ \Q\rb{\omega} = \Q\rb{\sqrt{-3}}, \qquad \Q\rb{\sqrt[3]{2}} = \cb{a + b\sqrt[3]{2} + c\sqrt[3]{4} \mid a, b, c \in \Q}. $$
\end{example*}

\begin{remark*}
For any splitting field of $ f $, there is always a natural inclusion group homomorphism
$$ \rho : G \hookrightarrow S\rb{\lambda_1, \dots, \lambda_n}, $$
where $ S\rb{\lambda_1, \dots, \lambda_n} $ is the group of permutations of the roots of $ f = x^n + a_1x^{n - 1} + \dots + a_n $.
\begin{itemize}
\item If $ \sigma \in G $, $ f\rb{\lambda} = 0 $, so $ \lambda^n + a_1\lambda^{n - 1} + \dots + a_n = 0 $.
$$ 0 = \sigma\rb{0} = \sigma\rb{\lambda^n + a_1\lambda^{n - 1} + \dots + a_n} = \sigma\rb{\lambda}^n + a_1\sigma\rb{\lambda}^{n - 1} + \dots + a_n. $$
\item $ \rho $ is injective. If for all $ i $, $ \sigma\rb{\lambda_i} = \lambda_i $, then $ \sigma = id $ on $ K\rb{\lambda_1, \dots, \lambda_n} = L $.
\end{itemize}
\end{remark*}

The fundamental theorem and remark gives $ G = \mathfrak{S}_3 $.

\lecture{4}{Thursday}{17/01/19}

\begin{definition}
$ K \subset L $ is \textbf{finite} if $ L $ is finite-dimensional as a vector space over $ K $. The \textbf{degree} of $ L $ over $ K $ is $ \sb{L : K} = \dim_{K}\rb{L} $.
\end{definition}

Two things about this.

\begin{theorem}[Tower law]
\label{thm:towerlaw}
Let $ K \subset L \subset F $. Then $ \sb{F : K} = \sb{F : L}\sb{L : K} $.
\end{theorem}

\begin{theorem}
\label{thm:degree}
Suppose $ f\rb{x} \in K\sb{x} $ is irreducible of degree $ d = \deg\rb{f} $ and $ L = K\rb{\lambda} $ where $ f\rb{\lambda} = 0 $, then $ \sb{K\rb{\lambda} : K} = d $.
\end{theorem}

\begin{example*}
$$ K = \Q\rb{\sqrt[3]{2}} = \cb{a + b\sqrt[3]{2} + c\sqrt[3]{4} \mid a, b, c \in \Q} $$
is a field, and $ \sb{K : \Q} = 3 $.
\end{example*}

\begin{example*}
Let $ L = \Q\rb{\sqrt[3]{2}, \omega} $ be the splitting field of $ x^3 - 2 $ over $ \Q $. The lattice of subfields is
$$
\begin{tikzcd}
& & L & \\
\Q\rb{\sqrt[3]{2}} \arrow[dash]{urr}{2} & \Q\rb{\omega\sqrt[3]{2}} \arrow[dash]{ur}{2} & \Q\rb{\omega^2\sqrt[3]{2}} \arrow[dash]{u}{2} & \\
& & & \Q\rb{\omega} \arrow[dash, swap]{uul}{3} \\
& & \Q \arrow[dash]{uull}{3} \arrow[dash]{uul}{3} \arrow[dash]{uu}{3} \arrow[dash, swap]{ur}{2} &
\end{tikzcd}.
$$
Then
$$ \Q\rb{\sqrt[3]{2} + \omega} = L, \qquad \Q\rb{\omega^2\sqrt[3]{2}} \cap \Q\rb{\omega\sqrt[3]{2}} = \Q, \qquad \Q\rb{\sqrt[3]{2}, \omega\sqrt[3]{2}} = L. $$
(Exercise) What is $ \sb{L : \Q\rb{\sqrt[3]{2}}} $? Note that $ L = \Q\rb{\sqrt[3]{2}}\rb{\sqrt{-3}} $. Could $ \sqrt{-3} \in \Q\rb{\sqrt[3]{2}} $? Consider $ x^2 + 3 \in \Q\rb{\sqrt[3]{2}}\sb{x} $. By the tower law,
$$
\begin{cases}
\sb{L : \Q} = \sb{L : \Q\rb{\omega}}\sb{\Q\rb{\omega} : \Q} = 2\sb{L : \Q\rb{\omega}} & \implies 2 \mid \sb{L : \Q} \\
\sb{L : \Q} = \sb{L : \Q\rb{\sqrt[3]{2}}}\sb{\Q\rb{\sqrt[3]{2}} : \Q} = 3\sb{L : \Q\rb{\sqrt[3]{2}}} & \implies 3 \mid \sb{L : \Q}
\end{cases}
\qquad \implies \qquad 6 \mid \sb{L : \Q}.
$$
\begin{itemize}
\item Either $ x^2 + 3 $ is irreducible over $ \Q\rb{\sqrt[3]{2}} $, so by Theorem \ref{thm:degree} $ \sb{L : \Q\rb{\sqrt[3]{2}}} = 2 $ and $ \sb{L : \Q} = 6 $.
\item Or $ x^2 + 3 $ is not irreducible, so $ \Q\rb{\sqrt[3]{2}} = L $ and $ \sb{L : \Q} = 3 $, a contradiction.
\end{itemize}
Are there any other fields? Claim that there are no other fields. Suppose $ \Q \subsetneq K \subsetneq L $ is such a field. By the tower law $ \sb{K : \Q} = 2 $ or $ \sb{K : \Q} = 3 $.
\begin{itemize}
\item Suppose $ \sb{K : \Q} = 2 $.
$$
\begin{tikzcd}
& L & \\
& K\rb{\omega} \arrow[dash]{u} & \\
K \arrow[dash]{uur}{3} \arrow[dash]{ur} & & \Q\rb{\omega} \arrow[dash]{ul} \\
& \Q \arrow[dash]{ul}{2} \arrow[dash, swap]{ur}{2} &
\end{tikzcd}.
$$
\begin{itemize}
\item Either $ \omega \in K $, that is $ \Q\rb{\omega} \subset K $, so by the tower law $ \Q\rb{\omega} = K $.
\item Or $ \omega \notin K $ gives $ \sb{K\rb{\omega} : K} = 2 $, so $ \sb{K\rb{\omega} : \Q} = 4 $ contradicts the tower law for $ \Q \subset K\rb{\omega} \subset L $.
\end{itemize}
\item Suppose $ \sb{K : \Q} = 3 $.
$$
\begin{tikzcd}
L & \\
& K\rb{\sqrt[3]{2}} \arrow[dash]{ul} \\
K \arrow[dash]{uu}{2} \arrow[dash]{ur} & \\
\Q \arrow[dash]{u}{3} &
\end{tikzcd}.
$$
Claim that $ x^3 - 2 \in K\sb{x} $ splits. Suppose that it were irreducible, then $ \sb{K\rb{\sqrt[3]{2}} : K} = 3 $, which contradicts the tower law for $ K \subset K\rb{\sqrt[3]{2}} \subset L $. So it has a root in $ K $. Either $ \sqrt[3]{2} \in K $, $ \omega\sqrt[3]{2} \in K $, or $ \omega^2\sqrt[3]{2} \in K $. Thus $ \Q\rb{\sqrt[3]{2}} = K $, $ \Q\rb{\omega\sqrt[3]{2}} = K $, or $ \Q\rb{\omega^2\sqrt[3]{2}} = K $.
\end{itemize}
I want to prove that
$$ G = Aut_\Q\rb{L} = \cb{\sigma : L \to L \mid \sigma \mid_\Q = id_\Q} = \mathfrak{S}_3. $$
\end{example*}

\lecture{5}{Friday}{18/01/19}

\begin{proof}[Proof of Theorem \ref{thm:towerlaw}]
Suppose $ y_1, \dots, y_m \in F $ is a basis of $ F $ as a vector space over $ L $. Suppose $ x_1, \dots, x_n \in L $ is a basis of $ L $ as a vector space over $ K $. Claim that $ \cb{x_iy_j} $ is a basis of $ F $ over $ K $.
\begin{itemize}
\item $ \cb{x_iy_j} $ generates $ F $. Let $ z \in F $. There exist $ \mu_1, \dots, \mu_n \in L $ such that
\begin{equation}
\label{eq:1}
z = \mu_1y_1 + \dots + \mu_ny_n.
\end{equation}
$ \mu_j \in L $ so for all $ j $ there exists $ \lambda_{ij} \in K $ such that
\begin{equation}
\label{eq:2}
\mu_j = x_1\lambda_{1j} + \dots + x_m\lambda_{mj}.
\end{equation}
Plug in $ \rb{\ref{eq:2}} $ into $ \rb{\ref{eq:1}} $,
$$ z = \sum_{i, j} \lambda_{ij}x_iy_j. $$
\item $ \cb{x_iy_j} $ are linearly independent over $ K $. Suppose there exists $ \lambda_{ij} \in K $ such that
$$ 0 = \sum_{i, j} \lambda_{ij}x_iy_j = \sum_j \rb{\sum_i \lambda_{ij}x_i}y_j, $$
so for all $ j $, $ \sum_i \lambda_{ij}x_i = 0 $, so for all $ j $ and all $ i $, $ \lambda_{ij} = 0 $.
\end{itemize}
\end{proof}

\begin{example*}
To show $ G = \mathfrak{S}_3 $. Let $ \sigma = \onebytwo{1}{2} $. A basis of $ L / \Q $ is
$$ 1, \sqrt[3]{2}, \sqrt[3]{4}, \omega, \omega\sqrt[3]{2}, \omega\sqrt[3]{4}. $$
\begin{itemize}
\item $ \sigma\rb{1} = 1 $.
\item $ \sigma\rb{\sqrt[3]{2}} = \omega\sqrt[3]{2} $.
\item $ \sigma\rb{\omega\sqrt[3]{2}} = \sqrt[3]{2} $.
\item $ \sigma\rb{\sqrt[3]{4}} = \sigma\rb{\sqrt[3]{2} \cdot \sqrt[3]{2}} = \omega\sqrt[3]{2} \cdot \omega\sqrt[3]{2} = \omega^2\sqrt[3]{4} = \rb{-\omega - 1}\sqrt[3]{4} = -\omega\sqrt[3]{4} - \sqrt[3]{4} $.
\item $ \sigma\rb{\omega} = \sigma\rb{\omega\sqrt[3]{2} / \sqrt[3]{2}} = \sigma\rb{\omega\sqrt[3]{2}} / \sigma\rb{\sqrt[3]{2}} = \sqrt[3]{2} / \omega\sqrt[3]{2} = 1 / \omega = -1 - \omega $.
\item $ \sigma\rb{\omega\sqrt[3]{4}} = \sigma\rb{\omega\sqrt[3]{2} \cdot \sqrt[3]{2}} = \sigma\rb{\omega\sqrt[3]{2}} \cdot \sigma\rb{\sqrt[3]{2}} = \sqrt[3]{2} \cdot \omega\sqrt[3]{2} = \omega\sqrt[3]{4} $.
\end{itemize}
Thus
$$ \sigma =
\begin{pmatrix}
1 & 0 & 0 & -1 & 0 & 0 \\
0 & 0 & 0 & 0 & 1 & 0 \\
0 & 0 & -1 & 0 & 0 & 0 \\
0 & 0 & 0 & -1 & 0 & 0 \\
0 & 1 & 0 & 0 & 0 & 0 \\
0 & 0 & -1 & 0 & 0 & 1
\end{pmatrix}.
$$
A question is if there were $ \sigma \in G $ such that $ \rho\rb{\sigma} = \onebytwo{1}{2} $ then we have written the matrix of $ \sigma $ as a $ \Q $-linear map of $ L $ in a basis. But how to check that this $ \Q $-linear map is a field homomorphism? We know the Galois correspondence for extensions of degree two.
$$ Gal_{\Q\rb{\sqrt[3]{2}}}\rb{L}, Gal_{\Q\rb{\omega^2\sqrt[3]{2}}}\rb{L}, Gal_{\Q\rb{\omega\sqrt[3]{2}}}\rb{L} \subset G $$
contain an element of order two, and
$$
\begin{array}{rrl}
\rho : & Gal_{\Q\rb{\sqrt[3]{2}}}\rb{L} & \mapsto \onebytwo{2}{3} \\
& Gal_{\Q\rb{\omega^2\sqrt[3]{2}}}\rb{L} & \mapsto \onebytwo{1}{2} \\
& Gal_{\Q\rb{\omega\sqrt[3]{2}}}\rb{L} & \mapsto \onebytwo{1}{3}.
\end{array}
$$
The lattice of subgroups is
$$
\begin{tikzcd}
& & \cb{e} & \\
\ab{\onebytwo{2}{3}} \arrow[dash]{urr}{2} & \ab{\onebytwo{1}{2}} \arrow[dash]{ur}{2} & \ab{\onebytwo{1}{3}} \arrow[dash]{u}{2} & \\
& & & \onebythree{1}{2}{3} \arrow[dash, swap]{uul}{3} \\
& & G \arrow[dash]{uull}{3} \arrow[dash]{uul}{3} \arrow[dash]{uu}{3} \arrow[dash, swap]{ur}{2} &
\end{tikzcd}.
$$
$ \Q\rb{\omega} / \Q $ is the splitting field of $ x^2 + x + 1 $ and of $ x^2 + 3 $.
\end{example*}

We can learn the following. Let $ k \subset L $ be a splitting field. Consider $ k \subset K \subset L $. Then $ K \subset L $ is also a splitting field. The corresponding $ H \le G $ is the Galois group $ Gal_K\rb{L} $. On the other hand $ k \subset K $ is not always a splitting field. It is a splitting field if and only if the corresponding $ H \le G $ is a normal subgroup and in that case $ Gal_k\rb{K} = G / H $.

\pagebreak

\section{Elementary facts}

\lecture{6}{Tuesday}{22/01/19}

Let $ K \subset L $ and $ a \in L $. The \textbf{evaluation homomorphism}
$$ \function[e_a]{K\sb{x}}{K\sb{a} \subset L}{f\rb{x}}{f\rb{a}} $$
is a surjective ring homomorphism, where $ K\sb{a} $ is the smallest subring of $ L $ containing $ K $ and $ a $.

\begin{definition}
$ f\rb{x} = a_0x^n + \dots + a_n \in K\sb{x} $ is \textbf{monic} if $ a_0 = 1 $.
\end{definition}

\begin{lemma}
\hfill
\begin{itemize}
\item If $ a $ is transcendental, $ e_a $ is injective and it extends to $ \widetilde{e_a} : K\rb{x} \to K\rb{a} $, by
$$
\begin{tikzcd}
K\rb{x} \arrow{dr}{\widetilde{e_a}} & \\
K\sb{x} \arrow[subset]{u} \arrow[swap]{r}{e_a} & L
\end{tikzcd}.
$$
\item If $ a $ is algebraic, then $ Ker\rb{e_a} = \ab{f_a} $, where $ f_a \in K\sb{x} $ is irreducible, or prime, and unique if monic, then called the minimal polynomial of $ a \in L / K $. In this case
$$
\begin{tikzcd}
K\sb{x} \arrow{r}{e_a} & K\sb{a} \cong K\rb{a} \subset L \\
\dfrac{K\sb{x}}{\ab{f_a}} \arrow[subset]{u} \arrow{ur}{\sim}[swap]{\sb{e_a}}
\end{tikzcd}.
$$
\end{itemize}
\end{lemma}

\begin{proof}
There is nothing to prove.
\end{proof}

\begin{remark*}
Let $ g\rb{x} \in K\sb{x} $ and $ g\rb{a} \ne 0 $. Claim that $ 1 / g\rb{a} \in K\sb{a} $. Indeed $ \gcd\rb{f, g} = 1 $ in $ K\sb{x} $ and $ f \nmid g $. There exists $ \phi, \psi \in K\sb{x} $ such that $ f\phi + g\psi = 1 $ and $ g\rb{a}\psi\rb{a} = 1 $. All of this is saying
\begin{itemize}
\item $ K\sb{a} \cong K\rb{a} $, and
\item $ K\sb{x} / \ab{f_a} \cong K\rb{a} $.
\end{itemize}
\end{remark*}

Let
$$ Emb_K\rb{K\rb{a}, F} = \cb{\sigma : K\rb{a} \to F \mid \sigma \ \text{field homomorphism}, \ \sigma_K = id_K}, $$
where
$$
\begin{tikzcd}
& K\rb{a} \arrow[dotted]{dd}{\sigma} \\
k \arrow[subset]{ur}{\sigma} \arrow[subset, swap]{dr}{\sigma} & \\
& F
\end{tikzcd}.
$$

\begin{corollary}
For $ K \subset L $ and $ a \in L $ algebraic over $ K $,
\begin{itemize}
\item $ \sb{K\rb{a} : K} = \deg\rb{f_a} $, and
\item If $ K \subset F $ is an extension,
$$ Emb_K\rb{K\rb{a}, F} = \cb{b \in F \mid f_a\rb{b} = 0}. $$
\end{itemize}
\end{corollary}

\begin{proof}
Since $ K\rb{a} = K\sb{a} $, $ \sb{K\rb{a} : K} = \dim_K\rb{K\rb{a}} = \dim_K\sb{K\rb{a}} $. Suppose
$$ f\rb{x} = x^n + \mu_1x^{n - 1} + \dots + \mu_n \in K\sb{x} $$
is the minimal polynomial of $ a $ over $ K $. Claim that $ 1, \dots, a^{n - 1} $ is a basis of $ K\sb{a} $ over $ K $.
\begin{itemize}
\item The set generates $ K\sb{a} $. Let $ c \in K\sb{a} $. There exists $ g \in K\sb{x} $ such that $ g\rb{a} = c $. Long division gives
$$ g\rb{x} = f\rb{x}q\rb{x} + r\rb{x}, \qquad m = \deg\rb{r\rb{x}} < n. $$
Then $ r\rb{x} = \lambda_0 + \dots + \lambda_mx^m $ and $ g\rb{a} = r\rb{a} = \lambda_0 + \dots + \lambda_ma^m $.
\item The set is linearly independent, otherwise there exists
$$ g\rb{x} = \lambda_0 + \dots + \lambda_{n - 1}x^{n- 1} \in K\sb{x}, g\rb{a} = 0, $$
and $ f $ was not the minimal polynomial.
\end{itemize}
$ \sigma\rb{a} $ is a root of $ f $, since applying $ \sigma $ to $ f\rb{a} = 0 $ gives
$$ 0 = \sigma\rb{a^n + \mu_1a^{n - 1} + \dots + \mu_n} = \sigma\rb{a}^n + \mu_1^{n - 1}\sigma\rb{a}^{n - 1} + \dots + \mu_n = f\rb{\sigma\rb{a}}. $$
Vice versa, if $ b \in F $ is a root of $ f $,
$$ K\rb{b} \xleftarrow[\sim]{\sb{e_b}} \dfrac{K\sb{x}}{\ab{f}} \xrightarrow[\sim]{\sb{e_a}} K\rb{a}, $$
then $ \sigma = \sb{e_b}\sb{e_a}^{-1} $. Thus there is a one-to-one correspondence
$$
\begin{array}{rcl}
Emb_K\rb{K\rb{a}, F} & \leftrightarrow & \cb{b \in F \mid f\rb{b} = 0} \\
\sigma & \mapsto & \sigma\rb{a} \\
\sb{e_b}\sb{e_a}^{-1} & \mapsfrom & b
\end{array}.
$$
\end{proof}

\begin{corollary}
Let $ K $ be a field and $ f \in K\sb{x} $. Then there exists $ K \subset L $ such that $ f $ has a root in $ L $.
\end{corollary}

\begin{proof}
Take $ g $ a prime factor of $ f $. Take $ L = K\sb{x} / \ab{g} $. In here $ a = \sb{x} $ is a root of $ g $ hence a root of $ f $.
\end{proof}

\lecture{7}{Thursday}{24/01/19}

From now on in this course, we study field extensions $ K \subset L $, always assumed to be finite, so $ \sb{L : K} = \dim_K\rb{L} < \infty $.

\begin{remark*}
$ K \subset L $ is finite if and only if
\begin{itemize}
\item it is algebraic, that is for all $ a \in L $, $ a $ is algebraic over $ K $, and
\item it is finitely generated, that is there exist $ a_1, \dots, a_m \in L $ such that $ L = K\rb{a_1, \dots, a_m} $.
\end{itemize}
\end{remark*}

An important point of view is that we study all possible field homomorphisms
$$ Emb\rb{K, L} = \cb{\sigma : K \to L \mid \sigma \ \text{field homomorphism}}. $$
Often there is a field $ k \subset K, L $ in the background which we want to stay fixed, so
$$ Emb_k\rb{K, L} = \cb{\sigma : K \to L \mid \sigma \ \text{field homomorphism}, \ \sigma \mid_k = id_k}. $$

\begin{example*}
Let $ K = \Q\rb{\sqrt[3]{2}} $. The minimal polynomial of $ \sqrt[3]{2} $ is $ x^3 - 2 $. Let $ L = \Q\rb{\sqrt[3]{2}, \sqrt{-3}} $ be the splitting field of $ x^3 - 2 $. Then
$$ Emb_\Q\rb{K, L} = Emb\rb{K, L} = \cb{\text{roots of} \ x^3 - 2 \ \text{in} \ L} = \cb{\sqrt[3]{2}, \omega\sqrt[3]{2}, \omega^2\sqrt[3]{2}}. $$
\end{example*}

\begin{remark*}
Suppose $ k \subset K $. $ Emb_k\rb{K, K} = G = Gal_k\rb{K} $. Indeed every $ k $-homomorphism $ \sigma : K \to K $ is automatically invertible. We know $ \sigma $ is injective. $ \sigma $ is also surjective because $ \sigma $ is a $ k $-linear endomorphism of a finite-dimensional $ k $-vector space.
\end{remark*}

\section{Axiomatics}

\begin{proposition}
Fix $ k \subset K $ and $ k \subset L $. Then $ \#Emb_k\rb{K, L} \le \sb{K : k} $.
\end{proposition}

\begin{proof}
\hfill
\begin{itemize}[leftmargin=1in]
\item[Special case.] If $ K = k\rb{a} $, let $ f\rb{x} \in k\sb{x} $ be the minimal polynomial of $ a $. Then $ Emb_k\rb{k\rb{a}, L} $ is the roots of $ f\rb{x} $ in $ L $, so
$$ \#Emb_k\rb{K, L} = \#\cb{\text{roots}} \le \deg\rb{f} = \sb{k\rb{a} : k}, $$
as proved last time.
\item[General case.] If $ k = K $, nothing to do. Otherwise choose $ a \in K \setminus k $.
$$
\begin{tikzcd}
& & L \\
k \arrow[subset]{urr} \arrow[subset]{r} & k\rb{a} \arrow[dotted, swap]{ur}{y} \arrow[subset]{r} & K \arrow[dotted]{u}
\end{tikzcd}.
$$
Consider the restriction map
$$ \rho : Emb_k\rb{K, L} \to Emb_k\rb{k\rb{a}, L}. $$
Fix $ y \in Emb_k\rb{k\rb{a}, L} $. Then
$$ \rho^{-1}\rb{y} = \cb{x : K \to L \mid x \mid_{k\rb{a}} = id_{k\rb{a}}}. $$
Since $ \sb{k\rb{a} : k} > 1 $, by the tower law $ \sb{K : k\rb{a}} < \sb{K : k} $. By induction we may assume $ \#\rho^{-1}\rb{y} \le \sb{K : k\rb{a}} $. So
$$ \#Emb_k\rb{K, L} \le \sum_{y \in Emb_k\rb{k\rb{a}, L}} \#\rho^{-1}\rb{y} \le \sb{k\rb{a} : k}\sb{K : k\rb{a}} = \sb{K : k}, $$
by the tower law.
\end{itemize}
\end{proof}

\begin{proposition}
Suppose given two field extensions $ k \subset K $ and $ k \subset L $. Then there is a bigger field
$$
\begin{tikzcd}
& K \arrow[subset]{dr}{\phi_1} & \\
k \arrow[subset]{ur}{\sigma_1} \arrow[subset, swap]{dr}{\sigma_2} & & \Omega \\
& L \arrow[subset, swap]{ur}{\phi_2} &
\end{tikzcd}
$$
that contains both.
\end{proposition}

\begin{remark*}
\hfill
\begin{itemize}
\item More formally, suppose given $ \sigma_1 \in Emb\rb{k, K} $ and $ \sigma_2 \in Emb\rb{k, L} $, then there exists $ \Omega $, $ \phi_1 \in Emb\rb{K, \Omega} $, and $ \phi_2 \in Emb\rb{L, \Omega} $ such that $ \phi_1 \circ \sigma_1 = \phi_2 \circ \sigma_2 $.
\item I never said that $ \Omega $ is unique. For example, let $ K = \Q\rb{\sqrt[3]{2}} $ and $ L = \Q\rb{\sqrt[3]{2}} $. One choice is $ \Omega = k $. Another choice is $ \Omega = \Q\rb{\sqrt[3]{2}, \sqrt{-3}} $, where
$$
\begin{tikzcd}
& \Q\rb{\sqrt[3]{2}} \arrow[subset]{dr}{\phi_1 : \sqrt[3]{2} \mapsto \sqrt[3]{2}} & \\
\Q \arrow[subset]{ur}{\sigma} \arrow[subset, swap]{dr}{\sigma} & & \Q\rb{\sqrt[3]{2}, \sqrt{-3}} \\
& \Q\rb{\sqrt[3]{2}} \arrow[subset, swap]{ur}{\phi_2 : \sqrt[3]{2} \mapsto \sqrt{-3}} &
\end{tikzcd}.
$$
\end{itemize}
\end{remark*}

\end{document}